Ex05 tutorial not yet finshed.

Ex05.thy
@@ -1,4 +1,4 @@
-theory Ex05_Template
+theory Ex05
 imports Big_Step
 begin
 (*>*)
@@ -7,47 +7,158 @@ section {* Ex. 5.1 *}
 
 (* prove or disprove *)
 lemma "IF And b1 b2 THEN c1 ELSE c2 \<sim> IF b1 THEN IF b2 THEN c1 ELSE c2 ELSE c2"
-oops
+by (metis IfE IfFalse IfTrue bval.simps(3))
 
 (* prove or disprove *)
 lemma "WHILE And b1 b2 DO c \<sim> WHILE b1 DO WHILE b2 DO c"
 oops
 
+(* counterexample:
+  b1 = Less (V 0) (N 1)
+  b2 = Less (V 1) (N 1)
+  c = IF b1 THEN 0 ::= (N 1) ELSE 1 ::= (N 1) 
+  s = [0, 0]
+*)
+
+abbreviation "w1 b1 b2 c s t \<equiv> exec (WHILE And b1 b2 DO c) s t"
+abbreviation "w2 b1 b2 c s t \<equiv> exec (WHILE b1 DO WHILE b2 DO c) s t"
+
+values "{t. w1 (Less (V 0) (N 1)) (Less (V 1) (N 1)) (IF (Less (V 0) (N 1)) THEN 0 ::= (N 1) ELSE 1 ::= (N 1)) [0,0] t }"
+values "{t. w2 (Less (V 0) (N 1)) (Less (V 1) (N 1)) (IF (Less (V 0) (N 1)) THEN 0 ::= (N 1) ELSE 1 ::= (N 1)) [0,0] t }"
+
+(* attempt to be able to formally proof couterexamples
+
+
+lemma "(exec c l l') = ((c, nth l) \<Rightarrow> nth l')"
+proof
+  assume "(c, nth l) \<Rightarrow> nth l'"
+  thus "exec c l l'"
+    sledgehammer [full_types]
+
+
+lemma "\<not> (\<forall> b1 b2 c. WHILE And b1 b2 DO c \<sim> WHILE b1 DO WHILE b2 DO c)"
+proof (rule notI, elim allE)
+  let ?b1 = "Less (V 0) (N 1)"
+  let ?b2 = "Less (V 1) (N 1)"
+  let ?c = "IF ?b1 THEN 0 ::= (N 1) ELSE 1 ::= (N 1)" 
+  let ?s = "nth [0, 0]"
+  let ?t1 = "nth [1, 0]"
+  let ?t2 = "nth [1, 1]"
+  assume "(WHILE And ?b1 ?b2 DO ?c, ?s) \<Rightarrow> t =
+          (WHILE ?b1 DO WHILE ?b2 DO ?c, ?s) \<Rightarrow> t"
+  hence "False"
+    proof - 
+      have "(WHILE And ?b1 ?b2 DO ?c, ?s) \<Rightarrow> ?t1"
+
+. *)
+
 (* prove or disprove *)
 lemma "WHILE And b1 b2 DO c \<sim> WHILE b1 DO c; WHILE And b1 b2 DO c"
 oops
+
+(* counterexample:
+   b1 = (Less (V 0) (N 1)
+   b2 = (B False)
+   c = (0 :: (N 1))
+   s = [0]
+*)
+
+abbreviation "w3 b1 b2 c s t \<equiv> exec (WHILE b1 DO c; WHILE And b1 b2 DO c) s t"
+
+values "{t. w1 (Less (V 0) (N 1)) (B False) (0 ::= (N 1)) [0] t}"
+values "{t. w3 (Less (V 0) (N 1)) (B False) (0 ::= (N 1)) [0] t}"
+ 
 
 definition Or :: "bexp \<Rightarrow> bexp \<Rightarrow> bexp" where
   "Or b1 b2 = Not (And (Not b1) (Not b2))"
 
 (* prove or disprove *)
-lemma "WHILE Or b1 b2 DO c \<sim> WHILE Or b1 b2 DO c; WHILE b1 DO c"
-oops
 
+(* This is porvable. 
+
+TODO complete the proofs
+
+lemma not_or: "\<not>bval (Or b1 b2) s \<Longrightarrow> \<not>bval b1 s"
+by (metis Or_def bval.simps)
+
+lemma "\<lbrakk> (WHILE b DO c, s) \<Rightarrow> t \<rbrakk> \<Longrightarrow> \<not> bval b t"
+apply (induct rule: big_step.induct)
+apply (auto)
+
+apply blast
+
+
+
+lemma while_or: "\<lbrakk> (WHILE Or b1 b2 DO c, s) \<Rightarrow> t \<rbrakk> \<Longrightarrow> \<not>bval b1 t"
+proof -
+  assume 0: "(WHILE Or b1 b2 DO c, s) \<Rightarrow> t"
+  { assume 1: "\<not> bval (Or b1 b2) s"
+    with 0 have "s = t" by blast
+    with 1 have "\<not> bval b1 t" by (simp add: not_or) (* huh? *)
+  }
+  moreover
+  {
+    assume 1: "bval (Or b1 b2) s"
+    
+lemma "WHILE Or b1 b2 DO c \<sim> WHILE Or b1 b2 DO c; WHILE b1 DO c"
+
+proof -
+  { fix s t
+    assume 0: "(WHILE Or b1 b2 DO c, s) \<Rightarrow> t"
+    then have "bval b1 t = False" by (simp add: while_or)
+    then have "(WHILE b1 DO c, t) \<Rightarrow> t" by blast
+    with 0 have "(WHILE Or b1 b2 DO c; WHILE b1 DO c, s) \<Rightarrow> t" by blast
+  }
+  moreover
+  { fix s t
+    assume 1: "(WHILE Or b1 b2 DO c; WHILE b1 DO c, s) \<Rightarrow> t"
+    then obtain s' where 2: "(WHILE Or b1 b2 DO c, s) \<Rightarrow> s' \<and> (WHILE b1 DO c, s') \<Rightarrow> t" by blast
+    then have "bval b1 s' = False" by (fastsimp simp: while_or)
+    with 1 2 have "s' = t" by blast
+    with 2 have "(WHILE Or b1 b2 DO c, s) \<Rightarrow> t" by blast
+  }
+  ultimately show ?thesis by blast
+qed
+
+.
+oops
+*)
 
 
 section {* Ex. 5.2 *}
 
 lemma Semi_cong: "\<lbrakk> c1 \<sim> c1'; c2 \<sim> c2' \<rbrakk> \<Longrightarrow> c1; c2 \<sim> c1'; c2'"
-oops
+by auto
 
 lemma If_cong: "\<lbrakk>\<And>s. bval b s = bval b' s; c1 \<sim> c1'; c2 \<sim> c2' \<rbrakk>
    \<Longrightarrow> IF b THEN c1 ELSE c2 \<sim> IF b' THEN c1' ELSE c2'"
-oops
+by auto
+
+lemma While_cond: "\<lbrakk> (c1, s) \<Rightarrow> t; c1 = WHILE b DO c; \<And>s. bval b s = bval b' s; c \<sim> c' \<rbrakk>
+  \<Longrightarrow> (WHILE b' DO c', s) \<Rightarrow> t"
+by (induct c1 s t rule: big_step_induct) auto
 
 lemma While_cong: "\<lbrakk> \<And>s. bval b s = bval b' s; c \<sim> c' \<rbrakk>
   \<Longrightarrow> WHILE b DO c \<sim> WHILE b' DO c'"
-oops
+by (auto intro: While_cond)
 
 definition Do :: "com \<Rightarrow> bexp \<Rightarrow> com" ("DO _ WHILE _"  [0, 61] 61) where
-  "DO c WHILE b = SKIP" (* add real definition here! *)
+  "DO c WHILE b = c; WHILE b DO c"
 
 fun trans1 :: "com \<Rightarrow> com" where
-  "trans1 c = SKIP" (* add real definition here! *)
+  "trans1 SKIP = SKIP"
+| "trans1 (Assign x e) = Assign x e"
+| "trans1 (Semi c1 c2) = Semi (trans1 c1) (trans1 c2)"
+| "trans1 (If b c1 c2) = If b (trans1 c1) (trans1 c2)"
+| "trans1 (WHILE b DO c) = IF b THEN (DO (trans1 c) WHILE b) ELSE SKIP"
 
 lemma "trans1 c \<sim> c"
-oops
-
+proof (induct c)
+  case (While b c')
+  with While_cong have "WHILE b DO (trans1 c') \<sim> WHILE b DO c'" by auto
+  with While have "c'; (WHILE b DO c') \<sim> (trans1 c'); WHILE b DO (trans1 c')" by auto
+  thus ?case by (auto simp add: Do_def unfold_while)
+qed auto
 
 end
 (*>*)
